fix(Modal/Kripke): Fix some definition of rooted frames and manipulation (#257)

Foundation/Modal/Kripke/Hilbert/GL/MDP.lean
@@ -10,7 +10,7 @@ namespace Hilbert.GL
 
 namespace Kripke
 
-abbrev MDPCounterexampleFrame (F₁ F₂ : FiniteTransitiveTree) : FiniteTransitiveTree where
+abbrev mdpCounterexmpleFrame (F₁ F₂ : Frame) (r₁ r₂) [F₁.IsFiniteTree r₁] [F₂.IsFiniteTree r₂] : Frame where
   World := Unit ⊕ F₁.World ⊕ F₂.World
   Rel := λ x y =>
     match x, y with
@@ -19,94 +19,111 @@ abbrev MDPCounterexampleFrame (F₁ F₂ : FiniteTransitiveTree) : FiniteTransit
     | .inl _, .inl _ => False -- r ⊀ r
     | .inl _, _ => True -- r ≺ w₁ and r ≺ w₂ : w₁ ∈ M₁, w₂ ∈ M₂
     | _, _ => False
-  root := .inl PUnit.unit
-  root_rooted := by
+
+namespace mdpCounterexmpleFrame
+
+variable {F₁ F₂ : Frame} {r₁ : F₁.World} {r₂ : F₂.World} [F₁.IsFiniteTree r₁] [F₂.IsFiniteTree r₂]
+
+instance : Coe (F₁.World) (mdpCounterexmpleFrame F₁ F₂ r₁ r₂).World := ⟨Sum.inr ∘ Sum.inl⟩
+instance : Coe (F₂.World) (mdpCounterexmpleFrame F₁ F₂ r₁ r₂).World := ⟨Sum.inr ∘ Sum.inr⟩
+
+instance
+  {F₁ F₂ : Frame} {r₁ : F₁.World} {r₂ : F₂.World} [tree₁ : F₁.IsFiniteTree r₁] [tree₂ : F₂.IsFiniteTree r₂]
+  : (mdpCounterexmpleFrame F₁ F₂ r₁ r₂).IsFiniteTree (.inl ()) where
+  root_generates := by
     intro x hx;
     match x with
     | .inl x => contradiction;
-    | .inr _ => simp [Frame.Rel'];
+    | .inr _ =>
+      apply Relation.TransGen.single;
+      tauto;
   rel_assymetric := by
     intro x y hxy;
     match x, y with
-    | .inr (.inl x), .inr (.inl y) => apply F₁.rel_assymetric hxy;
-    | .inr (.inr x), .inr (.inr y) => apply F₂.rel_assymetric hxy;
+    | .inr (.inl x), .inr (.inl y) => exact tree₁.rel_assymetric hxy;
+    | .inr (.inr x), .inr (.inr y) => apply tree₂.rel_assymetric hxy;
     | .inl x, .inl y => contradiction;
     | .inl x, .inr y => simp;
   rel_transitive := by
     intro x y z hxy hyz;
     match x, y, z with
-    | .inr (.inl x), .inr (.inl y), .inr (.inl z) => apply F₁.rel_transitive hxy hyz;
-    | .inr (.inr x), .inr (.inr y), .inr (.inr z) => apply F₂.rel_transitive hxy hyz;
+    | .inr (.inl x), .inr (.inl y), .inr (.inl z) => apply tree₁.rel_transitive hxy hyz;
+    | .inr (.inr x), .inr (.inr y), .inr (.inr z) => apply tree₂.rel_transitive hxy hyz;
     | .inl _, .inr (.inr _), .inr (.inr _) => simp;
     | .inl _, .inr (.inl _), .inr (.inl _) => simp;
 
-namespace MDPCounterexampleFrame
+protected abbrev root : (mdpCounterexmpleFrame F₁ F₂ r₁ r₂).World := .inl ()
 
-variable {F₁ F₂ : FiniteTransitiveTree}
-
-instance : Coe (F₁.World) (MDPCounterexampleFrame F₁ F₂).World := ⟨Sum.inr ∘ Sum.inl⟩
-instance : Coe (F₂.World) (MDPCounterexampleFrame F₁ F₂).World := ⟨Sum.inr ∘ Sum.inr⟩
-
-def p_morphism₁ : F₁.toFrame →ₚ (MDPCounterexampleFrame F₁ F₂).toFrame where
+def pMorphism₁ : F₁ →ₚ (mdpCounterexmpleFrame F₁ F₂ r₁ r₂) where
   toFun x := .inr (.inl x)
   forth := by intro x y hxy; exact hxy;
-  back {x y} h := by
-    match y with
-    | .inr (.inl y) => use y;
+  back {x y} h := by match y with | .inr (.inl y) => use y;
 
-def p_morphism₂ : F₂.toFrame →ₚ (MDPCounterexampleFrame F₁ F₂).toFrame where
+def pMorphism₂ : F₂ →ₚ (mdpCounterexmpleFrame F₁ F₂ r₁ r₂) where
   toFun x := .inr (.inr x)
-  forth := by
-    intro x y hxy; exact hxy;
-  back {x y} h := by
-    match y with
-    | .inr (.inr y) => use y;
+  forth := by intro x y hxy; exact hxy;
+  back {x y} h := by match y with | .inr (.inr y) => use y;
 
-lemma through_original_root {x : (MDPCounterexampleFrame F₁ F₂).World} (h : (MDPCounterexampleFrame F₁ F₂).root ≺ x)
-  : (x = F₁.root ∨ (Sum.inr (Sum.inl F₁.root) ≺ x)) ∨ (x = F₂.root ∨ (Sum.inr (Sum.inr F₂.root) ≺ x)) := by
+lemma through_original_root {x : (mdpCounterexmpleFrame F₁ F₂ r₁ r₂).World} (h : mdpCounterexmpleFrame.root ≺ x)
+  : (x = r₁ ∨ (Sum.inr (Sum.inl r₁) ≺ x)) ∨ (x = r₂ ∨ (Sum.inr (Sum.inr r₂) ≺ x)) := by
   match x with
   | .inl x =>
-    have := (MDPCounterexampleFrame F₁ F₂).rel_irreflexive _ h;
+    have := (@Frame.IsTree.rel_irreflexive (mdpCounterexmpleFrame F₁ F₂ r₁ r₂) mdpCounterexmpleFrame.root _);
+    simp;
+    simp at this;
     contradiction;
   | .inr (.inl x) =>
-    by_cases h : x = F₁.root;
-    . subst h; left; tauto;
-    . left; right; exact p_morphism₁.forth $ F₁.root_rooted x h;
+    by_cases e : x = r₁;
+    . subst e; left; tauto;
+    . left; right;
+      exact pMorphism₁.forth $ by
+        apply Frame.IsRooted.direct_rooted_of_trans;
+        . exact Frame.IsTree.rel_transitive (r := r₁);
+        . assumption;
   | .inr (.inr x) =>
-    by_cases h : x = F₂.root;
+    by_cases h : x = r₂;
     . subst h; right; tauto;
-    . right; right; exact p_morphism₂.forth $ F₂.root_rooted x h;
+    . right; right;
+      exact pMorphism₂.forth $ by
+        apply Frame.IsRooted.direct_rooted_of_trans;
+        . exact Frame.IsTree.rel_transitive (r := r₂);
+        . assumption;
 
-end MDPCounterexampleFrame
+end mdpCounterexmpleFrame
 
-abbrev MDPCounterexampleModel (M₁ M₂ : FiniteTransitiveTreeModel) : FiniteTransitiveTreeModel where
-  toFiniteTransitiveTree := MDPCounterexampleFrame M₁.toFiniteTransitiveTree M₂.toFiniteTransitiveTree
+
+abbrev mdpCounterexmpleModel (M₁ M₂ : Model) (r₁ r₂) [M₁.IsFiniteTree r₁] [M₂.IsFiniteTree r₂] : Model where
+  toFrame := mdpCounterexmpleFrame (M₁.toFrame) (M₂.toFrame) r₁ r₂;
   Val := λ x a =>
     match x with
     | .inr (.inl x) => M₁.Val x a
     | .inr (.inr x) => M₂.Val x a
     | .inl _ => True
 
-namespace MDPCounterexampleModel
+namespace mdpCounterexmpleModel
 
-variable {M₁ M₂ : FiniteTransitiveTreeModel}
+variable {M₁ M₂ : Model} {r₁ : M₁.World} {r₂ : M₂.World} [tree₁ : M₁.IsFiniteTree r₁] [tree₂ : M₂.IsFiniteTree r₂]
 
-instance : Coe (M₁.World) (MDPCounterexampleModel M₁ M₂).World := ⟨Sum.inr ∘ Sum.inl⟩
-instance : Coe (M₂.World) (MDPCounterexampleModel M₁ M₂).World := ⟨Sum.inr ∘ Sum.inr⟩
+instance : Coe (M₁.World) (mdpCounterexmpleModel M₁ M₂ r₁ r₂).World := ⟨Sum.inr ∘ Sum.inl⟩
+instance : Coe (M₂.World) (mdpCounterexmpleModel M₁ M₂ r₁ r₂).World := ⟨Sum.inr ∘ Sum.inr⟩
 
-def p_morphism₁ : M₁.toModel →ₚ (MDPCounterexampleModel M₁ M₂).toModel := Model.PseudoEpimorphism.ofAtomic (MDPCounterexampleFrame.p_morphism₁) $ by
-  simp [MDPCounterexampleFrame.p_morphism₁];
+abbrev root : (mdpCounterexmpleModel M₁ M₂ r₁ r₂).World := mdpCounterexmpleFrame.root (F₁ := M₁.toFrame) (F₂ := M₂.toFrame) (r₁ := r₁) (r₂ := r₂)
 
-lemma modal_equivalence_original_world₁ {x : M₁.toModel.World} : ModalEquivalent (M₁ := M₁.toModel) (M₂ := (MDPCounterexampleModel M₁ M₂).toModel) x x := by
-  apply Kripke.Model.PseudoEpimorphism.modal_equivalence p_morphism₁;
+def pMorphism₁ : M₁ →ₚ (mdpCounterexmpleModel M₁ M₂ r₁ r₂) :=
+  Model.PseudoEpimorphism.ofAtomic (mdpCounterexmpleFrame.pMorphism₁ (F₁ := M₁.toFrame) (F₂ := M₂.toFrame) (r₁ := r₁) (r₂ := r₂)) $ by
+  simp [mdpCounterexmpleFrame.pMorphism₁];
 
-def p_morphism₂ : M₂.toModel →ₚ (MDPCounterexampleModel M₁ M₂).toModel := Model.PseudoEpimorphism.ofAtomic (MDPCounterexampleFrame.p_morphism₂) $ by
-  simp [MDPCounterexampleFrame.p_morphism₂];
+def pMorphism₂ : M₂ →ₚ (mdpCounterexmpleModel M₁ M₂ r₁ r₂) :=
+  Model.PseudoEpimorphism.ofAtomic (mdpCounterexmpleFrame.pMorphism₂ (F₁ := M₁.toFrame) (F₂ := M₂.toFrame) (r₁ := r₁) (r₂ := r₂)) $ by
+  simp [mdpCounterexmpleFrame.pMorphism₂];
 
-lemma modal_equivalence_original_world₂ {x : M₂.toModel.World} : ModalEquivalent (M₁ := M₂.toModel) (M₂ := (MDPCounterexampleModel M₁ M₂).toModel) x x := by
-  apply Kripke.Model.PseudoEpimorphism.modal_equivalence p_morphism₂;
+lemma modal_equivalence_original_world₁ {x : M₁.World} : ModalEquivalent (M₁ := M₁) (M₂ := (mdpCounterexmpleModel M₁ M₂ r₁ r₂)) x (↑x) := by
+  apply Kripke.Model.PseudoEpimorphism.modal_equivalence pMorphism₁;
 
-end MDPCounterexampleModel
+lemma modal_equivalence_original_world₂ {x : M₂.World} : ModalEquivalent (M₁ := M₂) (M₂ := (mdpCounterexmpleModel M₁ M₂ r₁ r₂)) x (↑x) := by
+  apply Kripke.Model.PseudoEpimorphism.modal_equivalence pMorphism₂;
+
+end mdpCounterexmpleModel
 
 end Kripke
 
@@ -122,40 +139,47 @@ lemma MDP_Aux (h : (□''X) *⊢[Hilbert.GL]! □φ₁ ⋎ □φ₂) : (□''X) 
     by_contra hC;
     have ⟨h₁, h₂⟩ : (Hilbert.GL ⊬ ⊡c ➝ φ₁) ∧ (Hilbert.GL ⊬ ⊡c ➝ φ₂) := not_or.mp hC;
 
-    obtain ⟨M₁, hM₁⟩ := Hilbert.GL.Kripke.iff_unprovable_exists_unsatisfies_FiniteTransitiveTree.mp h₁;
-    obtain ⟨M₂, hM₂⟩ := Hilbert.GL.Kripke.iff_unprovable_exists_unsatisfies_FiniteTransitiveTree.mp h₂;
+    obtain ⟨M₁, r₁, _, hM₁⟩ := Hilbert.GL.Kripke.iff_unprovable_exists_unsatisfies_FiniteTransitiveTree.mp h₁;
+    obtain ⟨M₂, r₂, _, hM₂⟩ := Hilbert.GL.Kripke.iff_unprovable_exists_unsatisfies_FiniteTransitiveTree.mp h₂;
 
-    replace hM₁ := @Kripke.MDPCounterexampleModel.modal_equivalence_original_world₁ (M₁ := M₁) (M₂ := M₂) M₁.root (⊡c ⋏ ∼φ₁) |>.mp $ Formula.Kripke.Satisfies.not_imp.mp hM₁;
-    replace hM₂ := @Kripke.MDPCounterexampleModel.modal_equivalence_original_world₂ (M₁ := M₁) (M₂ := M₂) M₂.root (⊡c ⋏ ∼φ₂) |>.mp $ Formula.Kripke.Satisfies.not_imp.mp hM₂;
+    let M₀ := Kripke.mdpCounterexmpleModel M₁ M₂ r₁ r₂;
+    let r₀ := Kripke.mdpCounterexmpleModel.root (M₁ := M₁) (M₂ := M₂) (r₁ := r₁) (r₂ := r₂)
 
-    let M := Kripke.MDPCounterexampleModel M₁ M₂;
+    replace hM₁ : Satisfies M₀ ↑r₁ (⊡c ⋏ ∼φ₁) := Kripke.mdpCounterexmpleModel.modal_equivalence_original_world₁.mp (Formula.Kripke.Satisfies.not_imp.mp hM₁);
+    replace hM₂ : Satisfies M₀ ↑r₂ (⊡c ⋏ ∼φ₂) := Kripke.mdpCounterexmpleModel.modal_equivalence_original_world₂.mp (Formula.Kripke.Satisfies.not_imp.mp hM₂);
 
-    have hc : Satisfies M.toModel M.root (□c) := by
+    have hc : Satisfies M₀ r₀ (□c) := by
       intro x Rrx;
-      rcases Kripke.MDPCounterexampleFrame.through_original_root Rrx with ((rfl | Rrx) | (rfl | Rrx))
+      rcases Kripke.mdpCounterexmpleFrame.through_original_root Rrx with ((rfl | Rrx) | (rfl | Rrx))
       . exact (Satisfies.and_def.mp $ (Satisfies.and_def.mp hM₁).1).1;
       . exact (Satisfies.and_def.mp $ (Satisfies.and_def.mp hM₁).1).2 _ Rrx
       . exact (Satisfies.and_def.mp $ (Satisfies.and_def.mp hM₂).1).1;
       . exact (Satisfies.and_def.mp $ (Satisfies.and_def.mp hM₂).1).2 _ Rrx
-    have hp₁ : ¬(Satisfies M.toModel M.root (□φ₁)) := by
-      dsimp [Satisfies]; push_neg;
-      use .inr (.inl M₁.root);
+    have hp₁ : ¬(Satisfies M₀ r₀ (□φ₁)) := by
+      dsimp [Satisfies];
+      push_neg;
+      use (↑r₁);
       constructor;
-      . apply M.root_rooted; simp;
+      . tauto;
       . exact (Satisfies.and_def.mp hM₁).2;
-    have hp₂ : ¬(Satisfies M.toModel M.root (□φ₂)) := by
-      dsimp [Satisfies]; push_neg;
-      use .inr (.inr M₂.root);
+    have hp₂ : ¬(Satisfies M₀ r₀ (□φ₂)) := by
+      dsimp [Satisfies];
+      push_neg;
+      use (↑r₂);
       constructor;
-      . apply M.root_rooted; simp;
+      . tauto;
       . exact (Satisfies.and_def.mp hM₂).2;
-    have : ¬(Satisfies M.toModel M.root (□φ₁ ⋎ □φ₂)) := by
+    have : ¬(Satisfies M₀ r₀ (□φ₁ ⋎ □φ₂)) := by
       apply Satisfies.not_def.mpr;
       apply Satisfies.or_def.not.mpr;
       push_neg;
       exact ⟨hp₁, hp₂⟩;
-    have : ¬(Satisfies M.toModel M.root (□c ➝ (□φ₁ ⋎ □φ₂))) := _root_.not_imp.mpr ⟨hc, this⟩;
-    have := Hilbert.GL.Kripke.iff_unprovable_exists_unsatisfies_FiniteTransitiveTree.mpr ⟨M, this⟩;
+    have : ¬(Satisfies M₀ r₀ (□c ➝ (□φ₁ ⋎ □φ₂))) := _root_.not_imp.mpr ⟨hc, this⟩;
+    have : Hilbert.GL ⊬ □c ➝ □φ₁ ⋎ □φ₂ := Hilbert.GL.Kripke.iff_unprovable_exists_unsatisfies_FiniteTransitiveTree.mpr $ by
+      use M₀, r₀;
+      constructor;
+      . infer_instance;
+      . exact this;
     contradiction;
 
   rcases this with (h | h) <;> {
